C-verifier/src/Midend-IVL/Isabelle-UTP-Extended/AlgebraicLaws/Algebraic_Laws.thy
@@ -22,8 +22,13 @@ text \<open>In this section we introduce the semantic rules related to the diffe
       language, and this before any deductive proof verification activity or formal testing.\<close>
 
 theory Algebraic_Laws
-  imports "../../Isabelle-UTP/utp/utp_urel_laws"
+  imports 
+    UTP.utp_rel_laws
+    "../theories/Rel/utp_rel_more"
 begin
+
+syntax
+  "_assignment"     :: "svids \<Rightarrow> uexprs \<Rightarrow> '\<alpha> hrel"  (infixr ":==" 72)
 
 named_theorems symbolic_exec and symbolic_exec_assign_uop and symbolic_exec_assign_bop and
                symbolic_exec_assign_trop and symbolic_exec_assign_qtop and symbolic_exec_ex
@@ -34,134 +39,64 @@ subsection \<open>SKIP Laws\<close>
 text \<open>In this section we introduce the algebraic laws of programming related to the SKIP
       statement.\<close>
 
-lemma pre_skip_post: "(\<lceil>b\<rceil>\<^sub>< \<and> II) = (II \<and> \<lceil>b\<rceil>\<^sub>>)"
-  by rel_auto
-
-lemma skip_var:
-  fixes x :: "(bool \<Longrightarrow> '\<alpha>)"
-  shows "($x \<and> II) = (II \<and> $x\<acute>)"
-  by rel_auto
-
-lemma assign_r_alt_def [symbolic_exec]:
-  fixes x :: "('a \<Longrightarrow>'\<alpha>)"
-  shows "x :== v = II\<lbrakk>\<lceil>v\<rceil>\<^sub></$x\<rbrakk>"
-  by rel_auto
-
-lemma skip_r_alpha_eq:
-  "II = ($\<Sigma>\<acute> =\<^sub>u $\<Sigma>)"
-  by rel_auto
-
-lemma skip_r_refine_orig:
-  "(p \<Rightarrow> p) \<sqsubseteq> II"
-  by pred_blast
+declare assign_r_alt_def [symbolic_exec]
 
 lemma skip_r_eq[simp]: "\<lbrakk>II\<rbrakk>\<^sub>e (a, b) \<longleftrightarrow> a = b"
   by rel_auto
-
-lemma skip_refine_join:
-  "(p \<Rightarrow> q) \<sqsubseteq> II \<longleftrightarrow> `((p \<squnion> II) \<Rightarrow> q)`"
-  by pred_auto
- 
-lemma skip_refine_rel:
-  "`(II \<Rightarrow> (p \<Rightarrow> q))` \<Longrightarrow> (p \<Rightarrow> q) \<sqsubseteq> II"
-  by pred_auto
-  
-lemma skip_r_refine_pred:
-  "`(p \<Rightarrow> q)` \<Longrightarrow> (\<lceil>p\<rceil>\<^sub>< \<Rightarrow> \<lceil>q\<rceil>\<^sub>>) \<sqsubseteq> II"
-  by rel_auto
     
 subsection \<open>Assignment Laws\<close>
+
 text \<open>In this section we introduce the algebraic laws of programming related to the assignment
       statement.\<close>
 
-lemma "&v\<lbrakk>expr/v\<rbrakk> = [v \<mapsto>\<^sub>s expr] \<dagger> &v" ..
+declare usubst_lookup_upd_pr_var [symbolic_exec]
+declare usubst_lookup_upd [symbolic_exec]
+declare subst_var [symbolic_exec]
+declare assign_test [symbolic_exec]
+declare assign_r_comp [symbolic_exec]
+declare assign_twice [symbolic_exec]
+declare assign_rcond[symbolic_exec]
 
-lemma usubst_cancel[usubst,symbolic_exec]:
-  assumes 1:"weak_lens v"
-  shows "(&v)\<lbrakk>expr/v\<rbrakk> = expr"
-  using 1
-  by transfer' rel_auto
-
-lemma usubst_cancel_r[usubst,symbolic_exec]:
-  assumes 1:"weak_lens v"
-  shows "($v)\<lbrakk>\<lceil>expr\<rceil>\<^sub></$v\<rbrakk>= \<lceil>expr\<rceil>\<^sub><"
-  using 1
-  by  rel_auto
-
-lemma assign_test[symbolic_exec]:
-  assumes 1:"mwb_lens x"
-  shows     "(x :== \<guillemotleft>u\<guillemotright> ;; x :== \<guillemotleft>v\<guillemotright>) = (x :== \<guillemotleft>v\<guillemotright>)"
-  using 1
-  by (simp add: assigns_comp subst_upd_comp subst_lit usubst_upd_idem)
-
-lemma assign_r_comp[symbolic_exec]:
-  "(x :== u ;; P) = P\<lbrakk>\<lceil>u\<rceil>\<^sub></$x\<rbrakk>"
-  by (simp add: assigns_r_comp usubst)
-
-lemma assign_twice[symbolic_exec]:
-  assumes "mwb_lens x" and  "x \<sharp> f"
-  shows "(x :== e ;; x :== f) = (x :== f)"
-  using assms
-  by (simp add: assigns_comp usubst)
-
-lemma assign_commute:
-  assumes "x \<bowtie> y" "x \<sharp> f" "y \<sharp> e"
-  shows "(x :== e ;; y :== f) = (y :== f ;; x :== e)"
-  using assms
-  by (rel_auto, simp_all add: lens_indep_comm)
-
-lemma assign_cond:
-  fixes x :: "('a \<Longrightarrow> '\<alpha>)"
-  assumes "out\<alpha> \<sharp> b"
-  shows "(x :== e ;; (P \<triangleleft> b \<triangleright> Q)) =
-         ((x :== e ;; P) \<triangleleft>b\<lbrakk>\<lceil>e\<rceil>\<^sub></$x\<rbrakk>\<triangleright> (x :== e ;; Q))"
-  by rel_auto
-
-lemma assign_rcond[symbolic_exec]:
-  fixes x :: "('a \<Longrightarrow> '\<alpha>)"
-  shows "(x :== e ;; (P \<triangleleft> b \<triangleright>\<^sub>r Q)) = ((x :== e ;; P) \<triangleleft> (b\<lbrakk>e/x\<rbrakk>) \<triangleright>\<^sub>r (x :== e ;; Q))"
-  by rel_auto
-
-lemma assign_uop1[symbolic_exec_assign_uop]:
+lemma assign_uop1 [symbolic_exec_assign_uop]:
   assumes 1: "mwb_lens v"
   shows "(v :== e1 ;; v :== (uop F (&v))) = (v :== (uop F e1))"
   using 1
   by rel_auto
 
-lemma assign_bop1[symbolic_exec_assign_bop]:
+lemma assign_bop1 [symbolic_exec_assign_bop]:
   assumes 1: "mwb_lens v" and 2:"v \<sharp> e2"
   shows "(v :== e1 ;; v :== (bop bp (&v) e2)) = (v :== (bop bp e1 e2))"
   using 1 2
   by rel_auto
 
-lemma assign_bop2[symbolic_exec_assign_bop]:
+lemma assign_bop2 [symbolic_exec_assign_bop]:
   assumes 1: "mwb_lens v" and 2:"v \<sharp> e2"
   shows "(v :== e1 ;; v :== (bop bp e2 (&v))) = (v :== (bop bp e2 e1))"
   using 1 2
   by rel_auto
 
-lemma assign_trop1[symbolic_exec_assign_trop]:
+lemma assign_trop1 [symbolic_exec_assign_trop]:
   assumes 1: "mwb_lens v" and 2:"v \<sharp> e2" and 3:"v \<sharp> e3"
   shows "(v :== e1 ;; v :== (trop tp (&v) e2 e3)) =
          (v :== (trop tp e1 e2 e3))"
   using 1 2 3
   by rel_auto
 
-lemma assign_trop2[symbolic_exec_assign_trop]:
+lemma assign_trop2 [symbolic_exec_assign_trop]:
   assumes 1: "mwb_lens v" and 2:"v \<sharp> e2" and 3:"v \<sharp> e3"
   shows "(v :== e1 ;; v :== (trop tp e2 (&v) e3)) =
          (v :== (trop tp e2 e1 e3))"
   using 1 2 3
   by rel_auto
 
-lemma assign_trop3[symbolic_exec_assign_trop]:
+lemma assign_trop3 [symbolic_exec_assign_trop]:
   assumes 1: "mwb_lens v" and 2:"v \<sharp> e2" and 3:"v \<sharp> e3"
   shows "(v :== e1 ;; v :== (trop tp e2 e3 (&v))) =
          (v :== (trop tp e2 e3 e1))"
   using 1 2 3
   by rel_auto
 
-lemma assign_qtop1[symbolic_exec_assign_qtop]:
+lemma assign_qtop1 [symbolic_exec_assign_qtop]:
   assumes 1: "mwb_lens v" and 2:"v \<sharp> e2" and 3:"v \<sharp> e3" and 4:"v \<sharp> e4"
   shows "(v :== e1 ;; v :== (qtop tp (&v) e2 e3 e4)) =
          (v :== (qtop tp e1 e2 e3 e4))"
@@ -191,20 +126,10 @@ lemma assign_qtop4[symbolic_exec_assign_qtop]:
 
 lemma assign_cond_seqr_dist:
   "(v :== e ;; (P \<triangleleft> b \<triangleright> Q)) = ((v :== e ;; P) \<triangleleft> b\<lbrakk>\<lceil>e\<rceil>\<^sub></$v\<rbrakk> \<triangleright> (v :== e ;; Q))"
-  by rel_auto 
+  by (simp add: assign_r_comp usubst_condr)
+ 
 
 text \<open>In the sequel we find assignment laws proposed by Hoare\<close>
-
-lemma assign_vwb_skip:
-  assumes 1: "vwb_lens v"
-  shows "(v :== &v) = II"
-  by (simp add: assms skip_r_def usubst_upd_var_id)
-  
-lemma assign_simultaneous:
-  assumes  1: "vwb_lens v2"
-  and      2: "v1 \<bowtie> v2"
-  shows "(v1,v2 :== e, (&v2)) =  (v1 :== e)"
-  by (simp add: 1 2 usubst_upd_comm usubst_upd_var_id)
 
 lemma assign_seq:
   assumes  1: "vwb_lens var2"
@@ -291,288 +216,118 @@ lemma assign_cond_If_uop[symbolic_exec_assign_uop]:
   shows "(v :== E;;
          ((v :== uop F (&v)) \<triangleleft>uop F (&v)\<triangleright>\<^sub>r (v :== uop G (&v)))) =
          (v :== trop If (uop F E) (uop F E) (uop G E))"
-  using 1
-proof (rel_simp, transfer)
-  fix a :: 'a and b :: 'a and va :: "bool \<Longrightarrow> 'a" and Fa :: "bool \<Rightarrow> bool" and Ea :: "'a \<Rightarrow> bool" and Ga :: "bool \<Rightarrow> bool"
-  have "Fa (Ea a) \<longrightarrow> (Fa (Ea a) \<and> b = put\<^bsub>va\<^esub> a (Fa (Ea a)) \<or> \<not> Fa (Ea a) \<and> b = put\<^bsub>va\<^esub> a (Ga (Ea a))) \<and> b = put\<^bsub>va\<^esub> a (Fa (Ea a) \<or> \<not> Fa (Ea a) \<and> Ga (Ea a)) \<or> \<not> b = put\<^bsub>va\<^esub> a (Fa (Ea a) \<or> \<not> Fa (Ea a) \<and> Ga (Ea a)) \<and> (\<not> Fa (Ea a) \<or> \<not> b = put\<^bsub>va\<^esub> a (Fa (Ea a)))"
-    by presburger
-  then have "\<not> ((\<not> Fa (Ea a) \<or> \<not> b = put\<^bsub>va\<^esub> a (Fa (Ea a))) \<and> (Fa (Ea a) \<or> \<not> b = put\<^bsub>va\<^esub> a (Ga (Ea a)))) = (b = put\<^bsub>va\<^esub> a (Fa (Ea a) \<or> \<not> Fa (Ea a) \<and> Ga (Ea a)))"
-    by fastforce
-  then show "(Fa (Ea a) \<and> b = put\<^bsub>va\<^esub> a (Fa (Ea a)) \<or> \<not> Fa (Ea a) \<and> b = put\<^bsub>va\<^esub> a (Ga (Ea a))) = (b = put\<^bsub>va\<^esub> a (Fa (Ea a) \<or> \<not> Fa (Ea a) \<and> Ga (Ea a)))"
-    by meson
-qed
+  using 1 by (rel_simp)
 
 lemma assign_cond_If_bop[symbolic_exec_assign_bop]:
   assumes 1: "mwb_lens v" and 2:"v \<sharp> expr"
   shows "((v :== E);;
           ((v :== (bop F expr (&v))) \<triangleleft>bop F expr (&v)\<triangleright>\<^sub>r (v :== (bop G expr (&v))))) =
          (v :== (trop If (bop F expr E) (bop F expr E) (bop G expr E)))"
-  using 1 2
-proof (rel_simp, transfer)
-  fix a :: 'a and b :: 'a and va :: "bool \<Longrightarrow> 'a" and Fa :: "bool \<Rightarrow> bool" and Ea :: "'a \<Rightarrow> bool" and Ga :: "bool \<Rightarrow> bool"
-  have "Fa (Ea a) \<longrightarrow> (Fa (Ea a) \<and> b = put\<^bsub>va\<^esub> a (Fa (Ea a)) \<or> \<not> Fa (Ea a) \<and> b = put\<^bsub>va\<^esub> a (Ga (Ea a))) \<and> b = put\<^bsub>va\<^esub> a (Fa (Ea a) \<or> \<not> Fa (Ea a) \<and> Ga (Ea a)) \<or> \<not> b = put\<^bsub>va\<^esub> a (Fa (Ea a) \<or> \<not> Fa (Ea a) \<and> Ga (Ea a)) \<and> (\<not> Fa (Ea a) \<or> \<not> b = put\<^bsub>va\<^esub> a (Fa (Ea a)))"
-    by presburger
-  then have "\<not> ((\<not> Fa (Ea a) \<or> \<not> b = put\<^bsub>va\<^esub> a (Fa (Ea a))) \<and> (Fa (Ea a) \<or> \<not> b = put\<^bsub>va\<^esub> a (Ga (Ea a)))) = (b = put\<^bsub>va\<^esub> a (Fa (Ea a) \<or> \<not> Fa (Ea a) \<and> Ga (Ea a)))"
-    by fastforce
-  then show "(Fa (Ea a) \<and> b = put\<^bsub>va\<^esub> a (Fa (Ea a)) \<or> \<not> Fa (Ea a) \<and> b = put\<^bsub>va\<^esub> a (Ga (Ea a))) = (b = put\<^bsub>va\<^esub> a (Fa (Ea a) \<or> \<not> Fa (Ea a) \<and> Ga (Ea a)))"
-    by meson
-qed
+  using 1 2 by rel_simp
 
 lemma assign_cond_If_bop1[symbolic_exec_assign_bop]:
   assumes 1: "mwb_lens v" and 2:"v \<sharp> expr"
   shows "((v :== E);;
           ((v :== (bop F (&v) expr)) \<triangleleft>bop F (&v) expr\<triangleright>\<^sub>r (v :== (bop G (&v) expr)))) =
          (v :== (trop If (bop F E expr) (bop F E expr) (bop G E expr)))"
-  using 1 2
-proof (rel_simp, transfer)
-  fix a :: 'a and b :: 'a and va :: "bool \<Longrightarrow> 'a" and Fa :: "bool \<Rightarrow> bool" and Ea :: "'a \<Rightarrow> bool" and Ga :: "bool \<Rightarrow> bool"
-  have "Fa (Ea a) \<longrightarrow> (Fa (Ea a) \<and> b = put\<^bsub>va\<^esub> a (Fa (Ea a)) \<or> \<not> Fa (Ea a) \<and> b = put\<^bsub>va\<^esub> a (Ga (Ea a))) \<and> b = put\<^bsub>va\<^esub> a (Fa (Ea a) \<or> \<not> Fa (Ea a) \<and> Ga (Ea a)) \<or> \<not> b = put\<^bsub>va\<^esub> a (Fa (Ea a) \<or> \<not> Fa (Ea a) \<and> Ga (Ea a)) \<and> (\<not> Fa (Ea a) \<or> \<not> b = put\<^bsub>va\<^esub> a (Fa (Ea a)))"
-    by presburger
-  then have "\<not> ((\<not> Fa (Ea a) \<or> \<not> b = put\<^bsub>va\<^esub> a (Fa (Ea a))) \<and> (Fa (Ea a) \<or> \<not> b = put\<^bsub>va\<^esub> a (Ga (Ea a)))) = (b = put\<^bsub>va\<^esub> a (Fa (Ea a) \<or> \<not> Fa (Ea a) \<and> Ga (Ea a)))"
-    by fastforce
-  then show "(Fa (Ea a) \<and> b = put\<^bsub>va\<^esub> a (Fa (Ea a)) \<or> \<not> Fa (Ea a) \<and> b = put\<^bsub>va\<^esub> a (Ga (Ea a))) = (b = put\<^bsub>va\<^esub> a (Fa (Ea a) \<or> \<not> Fa (Ea a) \<and> Ga (Ea a)))"
-    by meson
-qed
+  using 1 2 by rel_simp
 
 lemma assign_cond_If_bop2[symbolic_exec_assign_bop]:
   assumes 1: "mwb_lens v" and 2:"v \<sharp> exp1" and 3:"v \<sharp> exp2"
   shows "((v :== E);;
           ((v :== (bop F (&v) exp1)) \<triangleleft>bop F (&v) exp1\<triangleright>\<^sub>r (v :== (bop G (&v) exp2)))) =
          (v :== (trop If (bop F E exp1) (bop F E exp1) (bop G E exp2)))"
-  using 1 2 3
-proof (rel_simp, transfer)
-  fix a :: 'a and b :: 'a and va :: "bool \<Longrightarrow> 'a" and Fa :: "bool \<Rightarrow> bool" and Ea :: "'a \<Rightarrow> bool" and Ga :: "bool \<Rightarrow> bool"
-  have "Fa (Ea a) \<longrightarrow> (Fa (Ea a) \<and> b = put\<^bsub>va\<^esub> a (Fa (Ea a)) \<or> \<not> Fa (Ea a) \<and> b = put\<^bsub>va\<^esub> a (Ga (Ea a))) \<and> b = put\<^bsub>va\<^esub> a (Fa (Ea a) \<or> \<not> Fa (Ea a) \<and> Ga (Ea a)) \<or> \<not> b = put\<^bsub>va\<^esub> a (Fa (Ea a) \<or> \<not> Fa (Ea a) \<and> Ga (Ea a)) \<and> (\<not> Fa (Ea a) \<or> \<not> b = put\<^bsub>va\<^esub> a (Fa (Ea a)))"
-    by presburger
-  then have "\<not> ((\<not> Fa (Ea a) \<or> \<not> b = put\<^bsub>va\<^esub> a (Fa (Ea a))) \<and> (Fa (Ea a) \<or> \<not> b = put\<^bsub>va\<^esub> a (Ga (Ea a)))) = (b = put\<^bsub>va\<^esub> a (Fa (Ea a) \<or> \<not> Fa (Ea a) \<and> Ga (Ea a)))"
-    by fastforce
-  then show "(Fa (Ea a) \<and> b = put\<^bsub>va\<^esub> a (Fa (Ea a)) \<or> \<not> Fa (Ea a) \<and> b = put\<^bsub>va\<^esub> a (Ga (Ea a))) = (b = put\<^bsub>va\<^esub> a (Fa (Ea a) \<or> \<not> Fa (Ea a) \<and> Ga (Ea a)))"
-    by meson
-qed
+  using 1 2 3 by rel_simp
 
 lemma assign_cond_If_bop4[symbolic_exec_assign_bop]:
   assumes 1: "mwb_lens v" and 2:"v \<sharp> exp1" and 3:"v \<sharp> exp2"
   shows "((v :== E);;
           ((v :== (bop F (&v) exp1)) \<triangleleft>bop F (&v) exp1\<triangleright>\<^sub>r (v :== (bop G exp2 (&v))))) =
          (v :== (trop If (bop F E exp1) (bop F E exp1) (bop G exp2 E)))"
-  using 1 2 3
-proof (rel_simp, transfer)
-  fix a :: 'a and b :: 'a and va :: "bool \<Longrightarrow> 'a" and Fa :: "bool \<Rightarrow> bool" and Ea :: "'a \<Rightarrow> bool" and Ga :: "bool \<Rightarrow> bool"
-  have "Fa (Ea a) \<longrightarrow> (Fa (Ea a) \<and> b = put\<^bsub>va\<^esub> a (Fa (Ea a)) \<or> \<not> Fa (Ea a) \<and> b = put\<^bsub>va\<^esub> a (Ga (Ea a))) \<and> b = put\<^bsub>va\<^esub> a (Fa (Ea a) \<or> \<not> Fa (Ea a) \<and> Ga (Ea a)) \<or> \<not> b = put\<^bsub>va\<^esub> a (Fa (Ea a) \<or> \<not> Fa (Ea a) \<and> Ga (Ea a)) \<and> (\<not> Fa (Ea a) \<or> \<not> b = put\<^bsub>va\<^esub> a (Fa (Ea a)))"
-    by presburger
-  then have "\<not> ((\<not> Fa (Ea a) \<or> \<not> b = put\<^bsub>va\<^esub> a (Fa (Ea a))) \<and> (Fa (Ea a) \<or> \<not> b = put\<^bsub>va\<^esub> a (Ga (Ea a)))) = (b = put\<^bsub>va\<^esub> a (Fa (Ea a) \<or> \<not> Fa (Ea a) \<and> Ga (Ea a)))"
-    by fastforce
-  then show "(Fa (Ea a) \<and> b = put\<^bsub>va\<^esub> a (Fa (Ea a)) \<or> \<not> Fa (Ea a) \<and> b = put\<^bsub>va\<^esub> a (Ga (Ea a))) = (b = put\<^bsub>va\<^esub> a (Fa (Ea a) \<or> \<not> Fa (Ea a) \<and> Ga (Ea a)))"
-    by meson
-qed
+  using 1 2 3 by rel_simp
 
 lemma assign_cond_If_bop5[symbolic_exec_assign_bop]:
   assumes 1: "mwb_lens v" and 2:"v \<sharp> exp1" and 3:"v \<sharp> exp2"
   shows "((v :== E);;
           ((v :== (bop F exp1 (&v))) \<triangleleft>bop F exp1 (&v)\<triangleright>\<^sub>r (v :== (bop G (&v) exp2)))) =
          (v :== (trop If (bop F exp1 E) (bop F exp1 E) (bop G E exp2)))"
-  using 1 2 3
-proof (rel_simp, transfer)
-  fix a :: 'a and b :: 'a and va :: "bool \<Longrightarrow> 'a" and Fa :: "bool \<Rightarrow> bool" and Ea :: "'a \<Rightarrow> bool" and Ga :: "bool \<Rightarrow> bool"
-  have "Fa (Ea a) \<longrightarrow> (Fa (Ea a) \<and> b = put\<^bsub>va\<^esub> a (Fa (Ea a)) \<or> \<not> Fa (Ea a) \<and> b = put\<^bsub>va\<^esub> a (Ga (Ea a))) \<and> b = put\<^bsub>va\<^esub> a (Fa (Ea a) \<or> \<not> Fa (Ea a) \<and> Ga (Ea a)) \<or> \<not> b = put\<^bsub>va\<^esub> a (Fa (Ea a) \<or> \<not> Fa (Ea a) \<and> Ga (Ea a)) \<and> (\<not> Fa (Ea a) \<or> \<not> b = put\<^bsub>va\<^esub> a (Fa (Ea a)))"
-    by presburger
-  then have "\<not> ((\<not> Fa (Ea a) \<or> \<not> b = put\<^bsub>va\<^esub> a (Fa (Ea a))) \<and> (Fa (Ea a) \<or> \<not> b = put\<^bsub>va\<^esub> a (Ga (Ea a)))) = (b = put\<^bsub>va\<^esub> a (Fa (Ea a) \<or> \<not> Fa (Ea a) \<and> Ga (Ea a)))"
-    by fastforce
-  then show "(Fa (Ea a) \<and> b = put\<^bsub>va\<^esub> a (Fa (Ea a)) \<or> \<not> Fa (Ea a) \<and> b = put\<^bsub>va\<^esub> a (Ga (Ea a))) = (b = put\<^bsub>va\<^esub> a (Fa (Ea a) \<or> \<not> Fa (Ea a) \<and> Ga (Ea a)))"
-    by meson
-qed
+  using 1 2 3 by rel_simp
 
 lemma assign_cond_If_bop6[symbolic_exec_assign_bop]:
   assumes 1: "mwb_lens v" and 2:"v \<sharp> exp1" and 3:"v \<sharp> exp2"
   shows "((v :== E);;
           ((v :== (bop F exp1 (&v))) \<triangleleft>bop F exp1 (&v)\<triangleright>\<^sub>r (v :== (bop G exp2 (&v))))) =
          (v :== (trop If (bop F exp1 E) (bop F exp1 E) (bop G exp2 E)))"
-  using 1 2 3
-proof (rel_simp, transfer)
-  fix a :: 'a and b :: 'a and va :: "bool \<Longrightarrow> 'a" and Fa :: "bool \<Rightarrow> bool" and Ea :: "'a \<Rightarrow> bool" and Ga :: "bool \<Rightarrow> bool"
-  have "Fa (Ea a) \<longrightarrow> (Fa (Ea a) \<and> b = put\<^bsub>va\<^esub> a (Fa (Ea a)) \<or> \<not> Fa (Ea a) \<and> b = put\<^bsub>va\<^esub> a (Ga (Ea a))) \<and> b = put\<^bsub>va\<^esub> a (Fa (Ea a) \<or> \<not> Fa (Ea a) \<and> Ga (Ea a)) \<or> \<not> b = put\<^bsub>va\<^esub> a (Fa (Ea a) \<or> \<not> Fa (Ea a) \<and> Ga (Ea a)) \<and> (\<not> Fa (Ea a) \<or> \<not> b = put\<^bsub>va\<^esub> a (Fa (Ea a)))"
-    by presburger
-  then have "\<not> ((\<not> Fa (Ea a) \<or> \<not> b = put\<^bsub>va\<^esub> a (Fa (Ea a))) \<and> (Fa (Ea a) \<or> \<not> b = put\<^bsub>va\<^esub> a (Ga (Ea a)))) = (b = put\<^bsub>va\<^esub> a (Fa (Ea a) \<or> \<not> Fa (Ea a) \<and> Ga (Ea a)))"
-    by fastforce
-  then show "(Fa (Ea a) \<and> b = put\<^bsub>va\<^esub> a (Fa (Ea a)) \<or> \<not> Fa (Ea a) \<and> b = put\<^bsub>va\<^esub> a (Ga (Ea a))) = (b = put\<^bsub>va\<^esub> a (Fa (Ea a) \<or> \<not> Fa (Ea a) \<and> Ga (Ea a)))"
-    by meson
-qed
+  using 1 2 3 by rel_simp
 
 lemma assign_cond_If_trop[symbolic_exec_assign_trop]:
   assumes 1: "mwb_lens v" and 2:"v \<sharp> exp1" and 3:"v \<sharp> exp2"
   shows "((v :== E);;
          ((v :== (trop F exp1 exp2 (&v))) \<triangleleft>trop F exp1 exp2 (&v)\<triangleright>\<^sub>r (v :== (trop G exp1 exp2 (&v))))) =
          (v :== (trop If (trop F exp1 exp2 E) (trop F exp1 exp2 E) (trop G exp1 exp2 E)))"
-  using 1 2 3
-proof (rel_simp, transfer)
-  fix a :: 'a and b :: 'a and va :: "bool \<Longrightarrow> 'a" and Fa :: "bool \<Rightarrow> bool" and Ea :: "'a \<Rightarrow> bool" and Ga :: "bool \<Rightarrow> bool"
-  have "Fa (Ea a) \<longrightarrow> (Fa (Ea a) \<and> b = put\<^bsub>va\<^esub> a (Fa (Ea a)) \<or> \<not> Fa (Ea a) \<and> b = put\<^bsub>va\<^esub> a (Ga (Ea a))) \<and> b = put\<^bsub>va\<^esub> a (Fa (Ea a) \<or> \<not> Fa (Ea a) \<and> Ga (Ea a)) \<or> \<not> b = put\<^bsub>va\<^esub> a (Fa (Ea a) \<or> \<not> Fa (Ea a) \<and> Ga (Ea a)) \<and> (\<not> Fa (Ea a) \<or> \<not> b = put\<^bsub>va\<^esub> a (Fa (Ea a)))"
-    by presburger
-  then have "\<not> ((\<not> Fa (Ea a) \<or> \<not> b = put\<^bsub>va\<^esub> a (Fa (Ea a))) \<and> (Fa (Ea a) \<or> \<not> b = put\<^bsub>va\<^esub> a (Ga (Ea a)))) = (b = put\<^bsub>va\<^esub> a (Fa (Ea a) \<or> \<not> Fa (Ea a) \<and> Ga (Ea a)))"
-    by fastforce
-  then show "(Fa (Ea a) \<and> b = put\<^bsub>va\<^esub> a (Fa (Ea a)) \<or> \<not> Fa (Ea a) \<and> b = put\<^bsub>va\<^esub> a (Ga (Ea a))) = (b = put\<^bsub>va\<^esub> a (Fa (Ea a) \<or> \<not> Fa (Ea a) \<and> Ga (Ea a)))"
-    by meson
-qed
+  using 1 2 3 by rel_simp
 
 lemma assign_cond_If_trop1[symbolic_exec_assign_trop]:
   assumes 1: "mwb_lens v" and 2:"v \<sharp> exp1" and 3:"v \<sharp> exp2"
   shows "((v :== E);;
           ((v :== (trop F exp1 (&v) exp2)) \<triangleleft>trop F exp1 (&v) exp2\<triangleright>\<^sub>r (v :== (trop G exp1 (&v) exp2)))) =
          (v :== (trop If (trop F exp1 E exp2) (trop F exp1 E exp2) (trop G exp1 E exp2)))"
-  using 1 2 3
-proof (rel_simp, transfer)
-  fix a :: 'a and b :: 'a and va :: "bool \<Longrightarrow> 'a" and Fa :: "bool \<Rightarrow> bool" and Ea :: "'a \<Rightarrow> bool" and Ga :: "bool \<Rightarrow> bool"
-  have "Fa (Ea a) \<longrightarrow> (Fa (Ea a) \<and> b = put\<^bsub>va\<^esub> a (Fa (Ea a)) \<or> \<not> Fa (Ea a) \<and> b = put\<^bsub>va\<^esub> a (Ga (Ea a))) \<and> b = put\<^bsub>va\<^esub> a (Fa (Ea a) \<or> \<not> Fa (Ea a) \<and> Ga (Ea a)) \<or> \<not> b = put\<^bsub>va\<^esub> a (Fa (Ea a) \<or> \<not> Fa (Ea a) \<and> Ga (Ea a)) \<and> (\<not> Fa (Ea a) \<or> \<not> b = put\<^bsub>va\<^esub> a (Fa (Ea a)))"
-    by presburger
-  then have "\<not> ((\<not> Fa (Ea a) \<or> \<not> b = put\<^bsub>va\<^esub> a (Fa (Ea a))) \<and> (Fa (Ea a) \<or> \<not> b = put\<^bsub>va\<^esub> a (Ga (Ea a)))) = (b = put\<^bsub>va\<^esub> a (Fa (Ea a) \<or> \<not> Fa (Ea a) \<and> Ga (Ea a)))"
-    by fastforce
-  then show "(Fa (Ea a) \<and> b = put\<^bsub>va\<^esub> a (Fa (Ea a)) \<or> \<not> Fa (Ea a) \<and> b = put\<^bsub>va\<^esub> a (Ga (Ea a))) = (b = put\<^bsub>va\<^esub> a (Fa (Ea a) \<or> \<not> Fa (Ea a) \<and> Ga (Ea a)))"
-    by meson
-qed
+  using 1 2 3 by rel_simp
 
 lemma assign_cond_If_trop2[symbolic_exec_assign_trop]:
   assumes 1: "mwb_lens v" and 2:"v \<sharp> exp1" and 3:"v \<sharp> exp2"
   shows "((v :== E);;
           ((v :== (trop F (&v) exp1 exp2)) \<triangleleft>trop F (&v) exp1 exp2\<triangleright>\<^sub>r (v :== (trop G (&v) exp1 exp2)))) =
          (v :== (trop If (trop F E exp1 exp2) (trop F E exp1 exp2) (trop G E exp1 exp2)))"
-  using 1 2 3
-proof (rel_simp, transfer)
-  fix a :: 'a and b :: 'a and va :: "bool \<Longrightarrow> 'a" and Fa :: "bool \<Rightarrow> bool" and Ea :: "'a \<Rightarrow> bool" and Ga :: "bool \<Rightarrow> bool"
-  have "Fa (Ea a) \<longrightarrow> (Fa (Ea a) \<and> b = put\<^bsub>va\<^esub> a (Fa (Ea a)) \<or> \<not> Fa (Ea a) \<and> b = put\<^bsub>va\<^esub> a (Ga (Ea a))) \<and> b = put\<^bsub>va\<^esub> a (Fa (Ea a) \<or> \<not> Fa (Ea a) \<and> Ga (Ea a)) \<or> \<not> b = put\<^bsub>va\<^esub> a (Fa (Ea a) \<or> \<not> Fa (Ea a) \<and> Ga (Ea a)) \<and> (\<not> Fa (Ea a) \<or> \<not> b = put\<^bsub>va\<^esub> a (Fa (Ea a)))"
-    by presburger
-  then have "\<not> ((\<not> Fa (Ea a) \<or> \<not> b = put\<^bsub>va\<^esub> a (Fa (Ea a))) \<and> (Fa (Ea a) \<or> \<not> b = put\<^bsub>va\<^esub> a (Ga (Ea a)))) = (b = put\<^bsub>va\<^esub> a (Fa (Ea a) \<or> \<not> Fa (Ea a) \<and> Ga (Ea a)))"
-    by fastforce
-  then show "(Fa (Ea a) \<and> b = put\<^bsub>va\<^esub> a (Fa (Ea a)) \<or> \<not> Fa (Ea a) \<and> b = put\<^bsub>va\<^esub> a (Ga (Ea a))) = (b = put\<^bsub>va\<^esub> a (Fa (Ea a) \<or> \<not> Fa (Ea a) \<and> Ga (Ea a)))"
-    by meson
-qed
+  using 1 2 3 by rel_simp
 
 lemma assign_cond_If_trop3[symbolic_exec_assign_trop]:
   assumes 1: "mwb_lens v" and 2:"v \<sharp> exp1" and 3:"v \<sharp> exp2" and 4:"v \<sharp> exp3" and 5:"v \<sharp> exp4"
   shows "((v :== E);;
           ((v :== (trop F exp1 exp2 (&v))) \<triangleleft>trop F exp1 exp2 (&v)\<triangleright>\<^sub>r (v :== (trop G exp3 exp4 (&v))))) =
          (v :== (trop If (trop F exp1 exp2 E) (trop F exp1 exp2 E) (trop G exp3 exp4 E)))"
-  using 1 2 3 4 5
-proof (rel_simp, transfer)
-  fix a :: 'a and b :: 'a and va :: "bool \<Longrightarrow> 'a" and Fa :: "bool \<Rightarrow> bool" and Ea :: "'a \<Rightarrow> bool" and Ga :: "bool \<Rightarrow> bool"
-  have "Fa (Ea a) \<longrightarrow> (Fa (Ea a) \<and> b = put\<^bsub>va\<^esub> a (Fa (Ea a)) \<or> \<not> Fa (Ea a) \<and> b = put\<^bsub>va\<^esub> a (Ga (Ea a))) \<and> b = put\<^bsub>va\<^esub> a (Fa (Ea a) \<or> \<not> Fa (Ea a) \<and> Ga (Ea a)) \<or> \<not> b = put\<^bsub>va\<^esub> a (Fa (Ea a) \<or> \<not> Fa (Ea a) \<and> Ga (Ea a)) \<and> (\<not> Fa (Ea a) \<or> \<not> b = put\<^bsub>va\<^esub> a (Fa (Ea a)))"
-    by presburger
-  then have "\<not> ((\<not> Fa (Ea a) \<or> \<not> b = put\<^bsub>va\<^esub> a (Fa (Ea a))) \<and> (Fa (Ea a) \<or> \<not> b = put\<^bsub>va\<^esub> a (Ga (Ea a)))) = (b = put\<^bsub>va\<^esub> a (Fa (Ea a) \<or> \<not> Fa (Ea a) \<and> Ga (Ea a)))"
-    by fastforce
-  then show "(Fa (Ea a) \<and> b = put\<^bsub>va\<^esub> a (Fa (Ea a)) \<or> \<not> Fa (Ea a) \<and> b = put\<^bsub>va\<^esub> a (Ga (Ea a))) = (b = put\<^bsub>va\<^esub> a (Fa (Ea a) \<or> \<not> Fa (Ea a) \<and> Ga (Ea a)))"
-    by meson
-qed
+  using 1 2 3 4 5 by rel_simp
 
 lemma assign_cond_If_trop4[symbolic_exec_assign_trop]:
   assumes 1: "mwb_lens v" and 2:"v \<sharp> exp1" and 3:"v \<sharp> exp2" and 4:"v \<sharp> exp3" and 5:"v \<sharp> exp4"
   shows "((v :== E);;
          ((v :== (trop F exp1 (&v) exp2)) \<triangleleft>trop F exp1 (&v) exp2\<triangleright>\<^sub>r (v :== (trop G exp3 (&v) exp4)))) =
          (v :== (trop If (trop F exp1 E exp2) (trop F exp1 E exp2) (trop G exp3 E exp4)))"
-  using 1 2 3 4 5
-proof (rel_simp, transfer)
-  fix a :: 'a and b :: 'a and va :: "bool \<Longrightarrow> 'a" and Fa :: "bool \<Rightarrow> bool" and Ea :: "'a \<Rightarrow> bool" and Ga :: "bool \<Rightarrow> bool"
-  have "Fa (Ea a) \<longrightarrow> (Fa (Ea a) \<and> b = put\<^bsub>va\<^esub> a (Fa (Ea a)) \<or> \<not> Fa (Ea a) \<and> b = put\<^bsub>va\<^esub> a (Ga (Ea a))) \<and> b = put\<^bsub>va\<^esub> a (Fa (Ea a) \<or> \<not> Fa (Ea a) \<and> Ga (Ea a)) \<or> \<not> b = put\<^bsub>va\<^esub> a (Fa (Ea a) \<or> \<not> Fa (Ea a) \<and> Ga (Ea a)) \<and> (\<not> Fa (Ea a) \<or> \<not> b = put\<^bsub>va\<^esub> a (Fa (Ea a)))"
-    by presburger
-  then have "\<not> ((\<not> Fa (Ea a) \<or> \<not> b = put\<^bsub>va\<^esub> a (Fa (Ea a))) \<and> (Fa (Ea a) \<or> \<not> b = put\<^bsub>va\<^esub> a (Ga (Ea a)))) = (b = put\<^bsub>va\<^esub> a (Fa (Ea a) \<or> \<not> Fa (Ea a) \<and> Ga (Ea a)))"
-    by fastforce
-  then show "(Fa (Ea a) \<and> b = put\<^bsub>va\<^esub> a (Fa (Ea a)) \<or> \<not> Fa (Ea a) \<and> b = put\<^bsub>va\<^esub> a (Ga (Ea a))) = (b = put\<^bsub>va\<^esub> a (Fa (Ea a) \<or> \<not> Fa (Ea a) \<and> Ga (Ea a)))"
-    by meson
-qed
+  using 1 2 3 4 5 by rel_simp
 
 lemma assign_cond_If_trop5[symbolic_exec_assign_trop]:
   assumes 1: "mwb_lens v" and 2:"v \<sharp> exp1" and 3:"v \<sharp> exp2" and 4:"v \<sharp> exp3" and 5:"v \<sharp> exp4"
   shows "((v :== E);;
           ((v :== (trop F (&v) exp1 exp2)) \<triangleleft>trop F (&v) exp1 exp2\<triangleright>\<^sub>r (v :== (trop G (&v) exp3 exp4)))) =
          (v :== (trop If (trop F E exp1 exp2) (trop F E exp1 exp2) (trop G E exp3 exp4)))"
-  using 1 2 3 4 5
-proof (rel_simp, transfer)
-  fix a :: 'a and b :: 'a and va :: "bool \<Longrightarrow> 'a" and Fa :: "bool \<Rightarrow> bool" and Ea :: "'a \<Rightarrow> bool" and Ga :: "bool \<Rightarrow> bool"
-  have "Fa (Ea a) \<longrightarrow> (Fa (Ea a) \<and> b = put\<^bsub>va\<^esub> a (Fa (Ea a)) \<or> \<not> Fa (Ea a) \<and> b = put\<^bsub>va\<^esub> a (Ga (Ea a))) \<and> b = put\<^bsub>va\<^esub> a (Fa (Ea a) \<or> \<not> Fa (Ea a) \<and> Ga (Ea a)) \<or> \<not> b = put\<^bsub>va\<^esub> a (Fa (Ea a) \<or> \<not> Fa (Ea a) \<and> Ga (Ea a)) \<and> (\<not> Fa (Ea a) \<or> \<not> b = put\<^bsub>va\<^esub> a (Fa (Ea a)))"
-    by presburger
-  then have "\<not> ((\<not> Fa (Ea a) \<or> \<not> b = put\<^bsub>va\<^esub> a (Fa (Ea a))) \<and> (Fa (Ea a) \<or> \<not> b = put\<^bsub>va\<^esub> a (Ga (Ea a)))) = (b = put\<^bsub>va\<^esub> a (Fa (Ea a) \<or> \<not> Fa (Ea a) \<and> Ga (Ea a)))"
-    by fastforce
-  then show "(Fa (Ea a) \<and> b = put\<^bsub>va\<^esub> a (Fa (Ea a)) \<or> \<not> Fa (Ea a) \<and> b = put\<^bsub>va\<^esub> a (Ga (Ea a))) = (b = put\<^bsub>va\<^esub> a (Fa (Ea a) \<or> \<not> Fa (Ea a) \<and> Ga (Ea a)))"
-    by meson
-qed
+  using 1 2 3 4 5 by rel_simp
 
 subsection \<open>Conditional Laws\<close>
+
 text \<open>In this section we introduce the algebraic laws of programming related to the conditional
       statement.\<close>
+
 named_theorems urel_cond
-lemma cond_idem[urel_cond]:
-  "(P \<triangleleft> b \<triangleright> P) = P"
-  by rel_auto
 
-lemma cond_symm:
-  "(P \<triangleleft> b \<triangleright> Q) = (Q \<triangleleft>\<not> b\<triangleright> P)"
-  by rel_auto
-
-lemma cond_assoc:
-  "(P \<triangleleft> b \<triangleright> (Q \<triangleleft> b \<triangleright> R)) = ((P \<triangleleft> b \<triangleright> Q) \<triangleleft> b \<triangleright>  R)"
-  by rel_auto
-
-lemma cond_distr[urel_cond]:
-  "((P \<triangleleft> b'\<triangleright> R) \<triangleleft> b \<triangleright> (Q \<triangleleft> b'\<triangleright> R))= ((P \<triangleleft> b \<triangleright> Q) \<triangleleft> b'\<triangleright> R)"
-  by rel_auto
-
-lemma cond_unit_T:
-  "(P \<triangleleft>true\<triangleright> Q) = P"
-  by auto
-
-lemma cond_unit_F:
-  "(P \<triangleleft>false\<triangleright> Q) = Q"
-  by auto
-
-lemma cond_and_T_integrate[urel_cond]:
-  "((P \<and> b) \<or> (Q \<triangleleft> b \<triangleright> R)) = ((P \<or> Q) \<triangleleft> b \<triangleright> R)"
-  by rel_auto
-
-lemma cond_L6[urel_cond]:
-  "(P \<triangleleft> b \<triangleright> (Q \<triangleleft> b \<triangleright> R)) = (P \<triangleleft> b \<triangleright> R)"
-  by rel_auto
-
-
-lemma cond_L7[urel_cond]:
-  "(P \<triangleleft> b \<triangleright> (P \<triangleleft> c \<triangleright> Q)) = (P \<triangleleft> b \<or> c \<triangleright> Q)"
-  by rel_auto
-
-lemma cond_and_distr[urel_cond]:
-  "((P \<and> Q) \<triangleleft> b \<triangleright> (R \<and> S)) = ((P \<triangleleft> b \<triangleright> R) \<and> (Q \<triangleleft> b \<triangleright> S))"
-  by rel_auto
-
-lemma cond_or_distr[urel_cond]:
-  "((P \<or> Q) \<triangleleft> b \<triangleright> (R \<or> S)) = ((P \<triangleleft> b \<triangleright> R) \<or> (Q \<triangleleft> b \<triangleright> S))"
-  by rel_auto
-
-lemma cond_imp_distr[urel_cond]:
-  "((P \<Rightarrow> Q) \<triangleleft> b \<triangleright> (R \<Rightarrow> S)) =
-   ((P \<triangleleft> b \<triangleright> R) \<Rightarrow> (Q \<triangleleft> b \<triangleright> S))"
-  by rel_auto
-
-lemma cond_eq_distr[urel_cond]:
-  "((P \<Leftrightarrow> Q) \<triangleleft> b \<triangleright> (R \<Leftrightarrow> S)) =
-   ((P \<triangleleft> b \<triangleright> R) \<Leftrightarrow> (Q \<triangleleft> b \<triangleright> S))"
-  by rel_auto
+declare cond_idem[urel_cond]
+declare cond_distr[urel_cond]
+declare cond_and_T_integrate [urel_cond]
+declare cond_L6 [urel_cond]
+declare cond_L7 [urel_cond]
+declare cond_and_distr [urel_cond]
+declare cond_or_distr[urel_cond]
+declare cond_imp_distr[urel_cond]
+declare cond_eq_distr[urel_cond]
 
 lemma cond_ueq_distr[urel_cond]:
   "((P =\<^sub>u Q) \<triangleleft> b \<triangleright> (R =\<^sub>u S)) =
    ((P \<triangleleft> b \<triangleright> R) =\<^sub>u (Q \<triangleleft> b \<triangleright> S))"
   by rel_auto
 
-lemma cond_conj_distr[urel_cond]:
-  "((P \<and> Q) \<triangleleft> b \<triangleright> (P \<and> S)) = (P \<and> (Q \<triangleleft> b \<triangleright> S))"
-  by rel_auto
-
-lemma cond_disj_distr [urel_cond]:
-  "((P \<or> Q) \<triangleleft> b \<triangleright> (P \<or> S)) = (P \<or> (Q \<triangleleft> b \<triangleright> S))"
-  by rel_auto
-
-lemma cond_neg[urel_cond]:
-  "\<not> (P \<triangleleft> b \<triangleright> Q) = ((\<not> P) \<triangleleft> b \<triangleright> (\<not> Q))"
-  by rel_auto
-
-lemma cond_conj[urel_cond]:
-  "(P \<triangleleft>b \<and> c\<triangleright> Q) = (P \<triangleleft> c \<triangleright> Q) \<triangleleft> b \<triangleright> Q"
-  by rel_auto
+declare cond_conj_distr [urel_cond]
+declare cond_disj_distr [urel_cond]
+declare cond_neg [urel_cond]
+declare cond_conj [urel_cond]
 
 (*IF Theorem by Hoare: It optimize nested IF*)
 theorem COND12[urel_cond]:
@@ -602,86 +357,35 @@ lemma cond_var_split[urel_cond]:
   "vwb_lens x \<Longrightarrow> (P\<lbrakk>true/x\<rbrakk> \<triangleleft>&x \<triangleright> P\<lbrakk>false/x\<rbrakk>) = P"
   by (rel_auto, (metis (full_types) vwb_lens.put_eq)+)
 
-lemma cond_seq_left_distr[urel_comp]:
-  "out\<alpha> \<sharp> b \<Longrightarrow> ((P \<triangleleft> b \<triangleright> Q) ;; R) = ((P ;; R) \<triangleleft> b \<triangleright> (Q ;; R))"
-  by rel_auto
+named_theorems urel_comp
 
-lemma cond_seq_right_distr[urel_comp]:
-  "in\<alpha> \<sharp> b \<Longrightarrow> (P ;; (Q \<triangleleft> b \<triangleright> R)) = ((P ;; Q) \<triangleleft> b \<triangleright> (P ;; R))"
-  by rel_auto
+declare cond_seq_left_distr [urel_comp]
+declare cond_seq_right_distr [urel_comp]
 
 subsection \<open>Sequential Laws\<close>
+
 text \<open>In this section we introduce the algebraic laws of programming related to the sequential
       composition of statements.\<close>
 
+declare seqr_exists_left [symbolic_exec]
+declare seqr_exists_right [symbolic_exec]
+declare seqr_left_zero [symbolic_exec_ex]
+declare seqr_right_zero [symbolic_exec_ex]
 
-lemma seqr_exists_left[symbolic_exec]:
-  "((\<exists> $x \<bullet> P) ;; Q) = (\<exists> $x \<bullet> (P ;; Q))"
-  by rel_auto
+declare seqr_or_distr [urel_comp]
 
-lemma seqr_exists_right[symbolic_exec]:
-  "(P ;; (\<exists> $x\<acute> \<bullet> Q)) = (\<exists> $x\<acute> \<bullet> (P ;; Q))"
-  by rel_auto
-
-lemma seqr_left_zero [simp, symbolic_exec_ex]:
-  "false ;; P = false"
-  by pred_auto
-
-lemma seqr_right_zero [simp, symbolic_exec_ex]:
-  "P ;; false = false"
-  by pred_auto
-
-lemma seqr_or_distr[urel_comp]:
-  "(P ;; (Q \<or> R)) = ((P ;; Q) \<or> (P ;; R))"
-  by rel_auto
-
-lemma seqr_unfold:
-  "(P ;; Q) = (\<^bold>\<exists> v \<bullet> P\<lbrakk>\<guillemotleft>v\<guillemotright>/$\<Sigma>\<acute>\<rbrakk> \<and> Q\<lbrakk>\<guillemotleft>v\<guillemotright>/$\<Sigma>\<rbrakk>)"
-  by rel_auto
-
-lemma seqr_middle:
-  assumes "vwb_lens x"
-  shows "(P ;; Q) = (\<^bold>\<exists> v \<bullet> P\<lbrakk>\<guillemotleft>v\<guillemotright>/$x\<acute>\<rbrakk> ;; Q\<lbrakk>\<guillemotleft>v\<guillemotright>/$x\<rbrakk>)"
-  using assms
-  apply (rel_auto robust)
-  apply (rename_tac xa P Q a b y)
-  apply (rule_tac x="get\<^bsub>xa\<^esub> y" in exI)
-  apply (rule_tac x="y" in exI)
-  apply (simp)
-done
-
-lemma seqr_left_one_point[urel_comp]:
-  assumes "vwb_lens x"
-  shows "((P \<and> $x\<acute> =\<^sub>u \<guillemotleft>v\<guillemotright>) ;; Q) = (P\<lbrakk>\<guillemotleft>v\<guillemotright>/$x\<acute>\<rbrakk> ;; Q\<lbrakk>\<guillemotleft>v\<guillemotright>/$x\<rbrakk>)"
-  using assms
-  by (rel_auto, metis vwb_lens_wb wb_lens.get_put)
-
-lemma seqr_right_one_point[urel_comp]:
-  assumes "vwb_lens x"
-  shows "(P ;; ($x =\<^sub>u \<guillemotleft>v\<guillemotright> \<and> Q)) = (P\<lbrakk>\<guillemotleft>v\<guillemotright>/$x\<acute>\<rbrakk> ;; Q\<lbrakk>\<guillemotleft>v\<guillemotright>/$x\<rbrakk>)"
-  using assms
-  by (rel_auto, metis vwb_lens_wb wb_lens.get_put)
-
-lemma seqr_insert_ident_left[urel_comp]:
-  assumes "vwb_lens x" "$x\<acute> \<sharp> P" "$x \<sharp> Q"
-  shows "(($x\<acute> =\<^sub>u $x \<and> P) ;; Q) = (P ;; Q)"
-  using assms
-  by (rel_auto, meson vwb_lens_wb wb_lens_weak weak_lens.put_get)
-
-lemma seqr_insert_ident_right[urel_comp]:
-  assumes "vwb_lens x" "$x\<acute> \<sharp> P" "$x \<sharp> Q"
-  shows "(P ;; ($x\<acute> =\<^sub>u $x \<and> Q)) = (P ;; Q)"
-  using assms
-  by (rel_auto, metis (no_types, hide_lams) vwb_lens_def wb_lens_def weak_lens.put_get)
-
-lemma seq_var_ident_lift[urel_comp]:
-  assumes "vwb_lens x" "$x\<acute> \<sharp> P" "$x \<sharp> Q"
-  shows "(($x\<acute> =\<^sub>u $x \<and> P) ;; ($x\<acute> =\<^sub>u $x \<and> Q)) = ($x\<acute> =\<^sub>u $x \<and> (P ;; Q))"
-  using assms
-  by (rel_auto, metis (no_types, lifting) vwb_lens_wb wb_lens_weak weak_lens.put_get)
+declare seqr_left_one_point [urel_comp]
+declare seqr_right_one_point[urel_comp]
+declare seqr_insert_ident_left[urel_comp]
+declare seqr_insert_ident_right[urel_comp]
+declare seq_var_ident_lift[urel_comp] 
 
 lemma seqr_skip: "II ;; C = C ;; II"
   by (metis seqr_left_unit seqr_right_unit)
+
+lemma post_str_rel: 
+  "(p\<Rightarrow>q) \<sqsubseteq> P \<Longrightarrow> `q\<Rightarrow>r` \<Longrightarrow> (p\<Rightarrow>r) \<sqsubseteq> P"
+  by pred_blast
 
 (*The rules SEQ6 SEQ7 related to SEQ and non-deterministic choice are missing for now*)
 
@@ -689,102 +393,13 @@ subsection \<open>While laws for normal designs\<close>
 
 text \<open>In this section we introduce the algebraic laws of programming related to the while
       statement.\<close>
-  
-lemma while_gfp_rel_def_alt:
-  "(while\<^sup>\<top> b do body od) = (\<nu> X \<bullet> bif b then (body ;; X) else SKIP\<^sub>r eif)"
-  unfolding from_until_gfp_rel_def while_gfp_rel_def 
-  by simp 
     
-lemma while_lfp_rel_def_alt:
-  "(while\<^sub>\<bottom> b do body od) = (\<mu> X \<bullet> bif b then (body ;; X) else SKIP\<^sub>r eif)"
-  unfolding from_until_lfp_rel_def while_lfp_rel_def 
-  by simp
-    
-theorem while_gfp_rel_unfold:
-  "while\<^sup>\<top> b do body od = (bif b then (body ;; while\<^sup>\<top> b do body od) else SKIP\<^sub>r eif)"
-proof -
-  have m:"mono (\<lambda>X. bif b then (body ;; X) else SKIP\<^sub>r eif)"
-    by (auto intro: monoI seqr_mono cond_mono)
-  have "(while\<^sup>\<top> b do body od) = (\<nu> X \<bullet> bif b then (body;; X) else SKIP\<^sub>r eif)"
-    by (simp add: while_gfp_rel_def_alt)
-  also have "... = (bif b then (body ;; (\<nu> X \<bullet> bif b then (body ;; X) else SKIP\<^sub>r eif)) else SKIP\<^sub>r eif)"
-    by (rule lfp_fixpoint[THEN sym, OF m])
-  also have "... = (bif b then (body ;; while\<^sup>\<top> b do body od) else SKIP\<^sub>r eif)"
-    by (simp add: while_gfp_rel_def_alt)
-  finally show ?thesis .
-qed
-  
-theorem while_lfp_rel_unfold:
-  "while\<^sub>\<bottom> b do body od = (bif b then (body;; while\<^sub>\<bottom> b do body od) else SKIP\<^sub>r eif)"
-proof -
-  have m:"mono (\<lambda>X. bif b then (body ;; X) else SKIP\<^sub>r eif)"
-    by (auto intro: monoI seqr_mono cond_mono)       
-  have "(while\<^sub>\<bottom> b do body od) = (\<mu> X \<bullet> bif b then (body ;; X) else SKIP\<^sub>r eif)"
-    by (simp add: while_lfp_rel_def_alt)
-  also have "... = (bif b then (body ;; (\<mu> X \<bullet> bif b then (body ;; X) else SKIP\<^sub>r eif)) else SKIP\<^sub>r eif)"
-     by (rule gfp_fixpoint[THEN sym, OF m]) 
-  also have "... = (bif b then (body ;; while\<^sub>\<bottom> b do body od) else SKIP\<^sub>r eif)"
-    by (simp add: while_lfp_rel_def_alt)
-  finally show ?thesis .
-qed
-    
-theorem while_lfp_rel_true: 
-  "while\<^sub>\<bottom> true do body od = (\<mu> X \<bullet> (body;; X))"
-  by (simp add: while_lfp_rel_def_alt alpha)
- 
-lemma while_lfp_rel_false:
-  "(while\<^sub>\<bottom> false do body od) = SKIP\<^sub>r"
-  by (simp add: while_lfp_rel_def_alt alpha gfp_const)
-
-theorem while_gfp_rel_false: 
- "while\<^sup>\<top> false do body od = SKIP\<^sub>r"
- by (simp add: while_gfp_rel_def_alt alpha lfp_const)
-
-theorem while_gfp_rel_non_termination: (*because of this lemma and the lemma utp_designs.design_top we do not use gfp for capturing termination *)
-  "while\<^sup>\<top> true do SKIP\<^sub>r od = false"
-  unfolding while_gfp_rel_def_alt  
-proof (rule lfp_eqI[of "(\<lambda>X. bif true then SKIP\<^sub>r ;; X else SKIP\<^sub>r eif)"] , goal_cases)
-  case 1
-  then show ?case by (auto intro: monoI seqr_mono cond_mono) 
-next
-  case 2
-  then show ?case by rel_simp  
-next
-  case 3
-  then show ?case by simp                      
-qed
-
-theorem while_lfp_rel_non_termination: 
-  "while\<^sub>\<bottom> true do SKIP\<^sub>r od = true"
-  unfolding while_lfp_rel_def_alt
-proof (rule gfp_eqI[of "(\<lambda>X. bif true then SKIP\<^sub>r ;; X else SKIP\<^sub>r eif)"] , goal_cases)
-  case 1
-  then show ?case by (auto intro: monoI seqr_mono cond_mono) 
-next
-  case 2
-  then show ?case  by rel_simp  
-next
-  case 3
-  then show ?case by simp                       
-qed    
-
-text \<open>An infinite loop with a feasible body corresponds to a program error (non-termination).\<close>
-
-theorem while_infinite: 
-  assumes is_in_abort_situation: "P ;; true\<^sub>h = true" 
-  shows "while\<^sub>\<bottom> true do P od = true"    
-  apply (simp add: while_lfp_rel_true)
-  apply (rule antisym)
-  apply (simp)
-  apply (rule gfp_upperbound)
-  apply (simp add: assms)
-  done
     
 subsection \<open>Other Iteration laws for relations\<close>
   
 theorem from_until_gfp_rel_alt_def:
   "from\<^sup>\<top> init until exit do body od = init ;; while\<^sup>\<top> \<not> exit do body od"
-  unfolding while_gfp_rel_def_alt from_until_gfp_rel_def 
+  unfolding while_def from_until_gfp_rel_def 
   by simp  
 
 lemma from_until_while_gfp_rel:
@@ -795,12 +410,12 @@ lemma from_until_while_gfp_rel:
 theorem from_until_gfp_rel_unfold:
   "from\<^sup>\<top> init until exit do body od = 
    init ;; (bif \<not> exit then (body;; while\<^sup>\<top> \<not> exit do body od) else SKIP\<^sub>r eif)"
-  unfolding from_until_gfp_rel_alt_def using while_gfp_rel_unfold[of "\<not>exit"]
-  by simp
+  unfolding from_until_gfp_rel_alt_def
+  by (metis while_unfold) 
     
 theorem from_until_lfp_rel_alt_def:
   "from\<^sub>\<bottom> init until exit do body od = init ;; while\<^sub>\<bottom> \<not> exit do body od"
-  unfolding while_lfp_rel_def_alt from_until_lfp_rel_def 
+  unfolding while_bot_def from_until_lfp_rel_def 
   by simp  
 
 lemma from_until_while_lfp_rel:
@@ -811,8 +426,8 @@ lemma from_until_while_lfp_rel:
 theorem from_until_lfp_rel_unfold:
   "from\<^sub>\<bottom> init until exit do body od = 
    init ;; (bif \<not> exit then (body;; while\<^sub>\<bottom> \<not> exit do body od) else SKIP\<^sub>r eif)"
-  unfolding from_until_lfp_rel_alt_def using while_lfp_rel_unfold[of "\<not>exit"]
-  by simp
+  unfolding from_until_lfp_rel_alt_def
+  by (metis while_bot_unfold) 
 
 theorem do_while_gfp_rel_alt_def:
   "do body while\<^sup>\<top> exit od = body ;; while\<^sup>\<top> exit do body od"
@@ -822,7 +437,7 @@ theorem do_while_gfp_rel_alt_def:
 theorem do_while_gfp_rel_unfold:
   "do body while\<^sup>\<top> exit od = 
    body ;; (bif exit then (body;; while\<^sup>\<top> exit do body od) else SKIP\<^sub>r eif)"
-  unfolding do_while_gfp_rel_alt_def using while_gfp_rel_unfold[of exit]
+  unfolding do_while_gfp_rel_alt_def using while_unfold[of exit]
   by simp
 
 theorem do_while_lfp_rel_alt_def:
@@ -833,7 +448,7 @@ theorem do_while_lfp_rel_alt_def:
 theorem do_while_lfp_rel_unfold:
   "do body while\<^sub>\<bottom> exit od = 
    body ;; (bif exit then (body;; while\<^sub>\<bottom> exit do body od) else SKIP\<^sub>r eif)"
-  unfolding do_while_lfp_rel_alt_def using while_lfp_rel_unfold[of exit]
+  unfolding do_while_lfp_rel_alt_def using while_bot_unfold[of exit]
   by simp    
 
 theorem for_gfp_rel_alt_def:
@@ -844,7 +459,7 @@ theorem for_gfp_rel_alt_def:
 theorem for_gfp_rel_unfold: 
   shows "for\<^sup>\<top> (init, exit, incr) do body od = 
          init ;; (bif exit then (body;;incr;;while\<^sup>\<top> exit do body ;; incr od) else SKIP\<^sub>r eif)"
-  unfolding for_gfp_rel_alt_def using while_gfp_rel_unfold 
+  unfolding for_gfp_rel_alt_def using while_unfold 
   by (metis seqr_assoc)
 
 theorem for_lfp_rel_alt_def:
@@ -855,79 +470,16 @@ theorem for_lfp_rel_alt_def:
 theorem for_lfp_rel_unfold:
   "for\<^sub>\<bottom> (init, exit, incr) do body od = 
    init ;; (bif exit then (body;;incr;;while\<^sub>\<bottom> exit do body ;; incr od) else SKIP\<^sub>r eif)"
-  unfolding for_lfp_rel_alt_def using while_lfp_rel_unfold 
+  unfolding for_lfp_rel_alt_def using while_bot_unfold 
   by (metis seqr_assoc)  
 
 subsection \<open>assume and assert laws\<close>
 
-lemma assume_twice[urel_comp]: "(b\<^sup>\<top> ;; c\<^sup>\<top>) = (b \<and> c)\<^sup>\<top>"
-  by rel_auto
+declare assume_seq [urel_comp]
+declare assert_seq [urel_comp]
+declare RA6 [urel_comp]
 
-lemma assert_twice[urel_comp]: "(b\<^sub>\<bottom> ;; c\<^sub>\<bottom>) = (b \<and> c)\<^sub>\<bottom>"
-  by rel_auto
-
-subsection \<open>Relation algebra laws\<close>
-
-theorem RA1: "(P ;; (Q ;; R)) = ((P ;; Q) ;; R)"
-  using seqr_assoc by auto
-
-theorem RA2: "(P ;; II) = P" "(II ;; P) = P"
-  by simp_all
-
-theorem RA3: "P\<^sup>-\<^sup>- = P"
-  by simp
-
-theorem RA4: "(P ;; Q)\<^sup>- = (Q\<^sup>- ;; P\<^sup>-)"
-  by simp
-
-theorem RA5: "(P \<or> Q)\<^sup>- = (P\<^sup>- \<or> Q\<^sup>-)"
-  by (rel_auto)
-
-theorem RA6[urel_comp]: "((P \<or> Q) ;; R) = ((P;;R) \<or> (Q;;R))"
-  using seqr_or_distl by blast
-
-theorem RA7: "((P\<^sup>- ;; (\<not>(P ;; Q))) \<or> (\<not>Q)) = (\<not>Q)"
-  by (rel_auto)
-
-subsection \<open>Refinement rules\<close>
-
-lemma reverse_impl_refine:
-  "`Q2 \<Rightarrow> Q1`  = (Q1 \<sqsubseteq> Q2)"
-  by pred_auto    
-  
-lemma pre_weak_rel:
-  assumes "`Pre \<Rightarrow> I`"
-  and     "(I \<Rightarrow> Post) \<sqsubseteq> P"
-  shows "(Pre \<Rightarrow> Post) \<sqsubseteq> P"
- using assms
-  by(rel_auto)
-    
-lemma post_str_rel: 
-  "(p\<Rightarrow>q) \<sqsubseteq> P \<Longrightarrow> `q\<Rightarrow>r` \<Longrightarrow> (p\<Rightarrow>r) \<sqsubseteq> P"
-  by pred_blast
-        
-lemma cond_refine_rel: 
-  assumes "(b \<and> p \<Rightarrow> q) \<sqsubseteq> C\<^sub>1" and "(\<not>b \<and> p \<Rightarrow> q)\<sqsubseteq> C\<^sub>2" 
-  shows "(p \<Rightarrow> q) \<sqsubseteq> (C\<^sub>1 \<triangleleft> b \<triangleright> C\<^sub>2)"
-  using assms by rel_auto
-    
-lemma cond_refine_pred: 
-  assumes "(\<lceil>b \<and> p\<rceil>\<^sub><\<Rightarrow> \<lceil>q\<rceil>\<^sub>>) \<sqsubseteq> C\<^sub>1" and "(\<lceil>\<not>b \<and> p\<rceil>\<^sub><\<Rightarrow> \<lceil>q\<rceil>\<^sub>>)\<sqsubseteq> C\<^sub>2" 
-  shows "(\<lceil>p\<rceil>\<^sub>< \<Rightarrow> \<lceil>q\<rceil>\<^sub>>) \<sqsubseteq> (C\<^sub>1 \<triangleleft> \<lceil>b\<rceil>\<^sub>< \<triangleright> C\<^sub>2)"
-  using assms by rel_auto
-
-lemma seq_refine_pred:
-  assumes "(\<lceil>p\<rceil>\<^sub>< \<Rightarrow> \<lceil>s\<rceil>\<^sub>>) \<sqsubseteq> f" and "(\<lceil>s\<rceil>\<^sub>< \<Rightarrow> \<lceil>q\<rceil>\<^sub>>) \<sqsubseteq> fa"
-  shows "(\<lceil>p\<rceil>\<^sub>< \<Rightarrow> \<lceil>q\<rceil>\<^sub>>) \<sqsubseteq> (f ;; fa)"
-  using assms by rel_auto
-   
-lemma seq_refine_unrest:
-  assumes "out\<alpha> \<sharp> p" "in\<alpha> \<sharp> q"
-  assumes "(p \<Rightarrow> \<lceil>s\<rceil>\<^sub>>) \<sqsubseteq> f" and "(\<lceil>s\<rceil>\<^sub>< \<Rightarrow> q) \<sqsubseteq> fa"
-  shows "(p \<Rightarrow> q) \<sqsubseteq> (f ;; fa)"
-  using assms by rel_blast    
-    
-lemmas skip_refine' = post_str_rel[OF skip_r_refine_orig]
+lemmas skip_refine' = post_str_rel[OF skip_r_refine]
 
 end
 
